weakened fullabs
tried to prove a stronger version but met some obstacles.
1. requires excluded middle
2. stuck at equiv preservation.

FullAbs.v
@@ -24,44 +24,44 @@ Inductive Stmt: Type :=
 (* cannot handle func call: recursiveness? *)
 (* I even don't know how to handle it when recursing is not allowed! *)
 
-Fixpoint evalExpr (e: Expr) (varX: Z) (varY: Z): Z :=
+Fixpoint eval_expr (e: Expr) (varX: Z) (varY: Z): Z :=
   match e with
   | Num n => n
-  | Plus e1 e2 => (evalExpr e1 varX varY) + (evalExpr e2 varX varY)
-  | Minus e1 e2 => (evalExpr e1 varX varY) - (evalExpr e2 varX varY)
+  | Plus e1 e2 => (eval_expr e1 varX varY) + (eval_expr e2 varX varY)
+  | Minus e1 e2 => (eval_expr e1 varX varY) - (eval_expr e2 varX varY)
   | VarX => varX
   | VarY => varY
   | IteZero ec el er =>
-       let cond := (evalExpr ec varX varY) in
-       let l := (evalExpr el varX varY) in
-       let r := (evalExpr er varX varY) in
+       let cond := (eval_expr ec varX varY) in
+       let l := (eval_expr el varX varY) in
+       let r := (eval_expr er varX varY) in
        match cond with
        | Z0 => l
        | _ => r
        end
   end.
 
-Fixpoint evalStmt (s: Stmt) (varX: Z) (varY: Z) : list Z :=
+Fixpoint eval_stmt (s: Stmt) (varX: Z) (varY: Z) : list Z :=
   match s with
-  | LetX e1 e2 => let varX' := (evalExpr e1 varX varY) in 
-                    (evalStmt e2 varX' varY)
-  | LetY e1 e2 => let varY' := (evalExpr e1 varX varY) in
-                    (evalStmt e2 varX varY')
-  | Write e => [(evalExpr e varX varY)]
-  | Seq p q => (evalStmt p varX varY) ++ (evalStmt q varX varY)
+  | LetX e1 e2 => let varX' := (eval_expr e1 varX varY) in 
+                    (eval_stmt e2 varX' varY)
+  | LetY e1 e2 => let varY' := (eval_expr e1 varX varY) in
+                    (eval_stmt e2 varX varY')
+  | Write e => [(eval_expr e varX varY)]
+  | Seq p q => (eval_stmt p varX varY) ++ (eval_stmt q varX varY)
   end.
 
-Example E1: (Z.to_nat (evalExpr (Plus (Num 3) VarX) 2 3)) = 5.
+Example E1: (Z.to_nat (eval_expr (Plus (Num 3) VarX) 2 3)) = 5.
 Proof.
   auto.
 Qed.
 
-Example E2: (Z.to_nat (evalExpr (IteZero (Minus (Num 1) (Num 1)) VarX VarY) 3 5)) = 3.
-Proof. unfold evalExpr. auto.
+Example E2: (Z.to_nat (eval_expr (IteZero (Minus (Num 1) (Num 1)) VarX VarY) 3 5)) = 3.
+Proof. unfold eval_expr. auto.
 Qed.
 
-Example E3: ((evalStmt (Seq (LetX (Num 1) (LetY (Num 2) (Write VarX))) (Write VarY)) 3 4) = [1%Z; 4%Z]).
-Proof. unfold evalStmt. simpl. reflexivity.
+Example E3: ((eval_stmt (Seq (LetX (Num 1) (LetY (Num 2) (Write VarX))) (Write VarY)) 3 4) = [1%Z; 4%Z]).
+Proof. unfold eval_stmt. simpl. reflexivity.
 Qed.
 
 Inductive Instr: Type := 
@@ -79,38 +79,38 @@ Inductive Instr: Type :=
   | ISwap: Instr.
 
 (* return: stack & write events *)
-Fixpoint evalInstr (prog: (list Instr)) (stack: list Z) (regX: Z) (regY: Z): option (list Z * list Z * (Z*Z)) :=
+Fixpoint eval_instr (prog: (list Instr)) (stack: list Z) (regX: Z) (regY: Z): option (list Z * list Z * (Z*Z)) :=
   match (prog, stack) with
   | (nil, result) => Some(result, [], (regX, regY))
-  | (IPlus :: prog', n1 :: n2 :: rest) => (evalInstr prog' ((n2 + n1)%Z :: rest) regX regY)
-  | (IMinus :: prog', n1 :: n2 :: rest) => (evalInstr prog' ((n2 - n1)%Z :: rest) regX regY)
-  | (IWrite :: prog', n :: rest) => match (evalInstr prog' stack regX regY) with
+  | (IPlus :: prog', n1 :: n2 :: rest) => (eval_instr prog' ((n2 + n1)%Z :: rest) regX regY)
+  | (IMinus :: prog', n1 :: n2 :: rest) => (eval_instr prog' ((n2 - n1)%Z :: rest) regX regY)
+  | (IWrite :: prog', n :: rest) => match (eval_instr prog' stack regX regY) with
                                     | Some(stack', evt', (regX', regY')) => Some(stack', n :: evt', (regX', regY'))
                                     | None => None
                                     end
   | (ICondPick :: prog', cond :: l :: r :: rest) =>
     match cond with
-    | Z0 => (evalInstr prog' (l :: rest) regX regY)
-    | _ => (evalInstr prog' (r :: rest) regX regY)
+    | Z0 => (eval_instr prog' (l :: rest) regX regY)
+    | _ => (eval_instr prog' (r :: rest) regX regY)
     end
-  | (ILoadX :: prog', n :: rest) => (evalInstr prog' rest n regY)
-  | (ILoadY :: prog', n :: rest) => (evalInstr prog' rest regX n)
-  | (IStoreX :: prog', _) => (evalInstr prog' (regX :: stack) regX regY)
-  | (IStoreY :: prog', _) => (evalInstr prog' (regY :: stack) regX regY)
-  | ((IStoreImm imm) :: prog', _) => (evalInstr prog' (imm :: stack) regX regY)
-  | (IPop :: prog', n :: rest) => (evalInstr prog' rest regX regY)
-  | (IDup :: prog', n :: rest) => (evalInstr prog' (n :: n :: rest) regX regY)
-  | (ISwap :: prog', n1 :: n2 :: rest) => (evalInstr prog' (n2 :: n1 :: rest) regX regY)
+  | (ILoadX :: prog', n :: rest) => (eval_instr prog' rest n regY)
+  | (ILoadY :: prog', n :: rest) => (eval_instr prog' rest regX n)
+  | (IStoreX :: prog', _) => (eval_instr prog' (regX :: stack) regX regY)
+  | (IStoreY :: prog', _) => (eval_instr prog' (regY :: stack) regX regY)
+  | ((IStoreImm imm) :: prog', _) => (eval_instr prog' (imm :: stack) regX regY)
+  | (IPop :: prog', n :: rest) => (eval_instr prog' rest regX regY)
+  | (IDup :: prog', n :: rest) => (eval_instr prog' (n :: n :: rest) regX regY)
+  | (ISwap :: prog', n1 :: n2 :: rest) => (eval_instr prog' (n2 :: n1 :: rest) regX regY)
   | (_, _) => None
   end.
 
-Example InstrE1: (evalInstr (IDup :: IPlus :: nil) (1%Z :: nil) 0 0) = Some([2%Z], [], (0%Z,0%Z)).
+Example InstrE1: (eval_instr (IDup :: IPlus :: nil) (1%Z :: nil) 0 0) = Some([2%Z], [], (0%Z,0%Z)).
 Proof.
-  unfold evalInstr.
+  unfold eval_instr.
   auto.
 Qed.
 
-Example InstrE2: (evalInstr (IStoreX :: IWrite :: IPop :: nil) [] 3%Z 4%Z) = Some([], [3%Z], (3%Z, 4%Z)).
+Example InstrE2: (eval_instr (IStoreX :: IWrite :: IPop :: nil) [] 3%Z 4%Z) = Some([], [3%Z], (3%Z, 4%Z)).
 Proof.
   auto.
 Qed.
@@ -154,12 +154,12 @@ Fixpoint compile_stmt (s: Stmt): list Instr :=
 
 Compute compile_stmt (LetX (Num 1) (Write VarX)).
 
-Example CE1: evalInstr (compile_stmt (LetX (Num 1) (LetX (Num 2) (Write VarX)))) [] 0 0 = Some([], [2%Z], (0%Z, 0%Z)).
+Example CE1: eval_instr (compile_stmt (LetX (Num 1) (LetX (Num 2) (Write VarX)))) [] 0 0 = Some([], [2%Z], (0%Z, 0%Z)).
 Proof. simpl. reflexivity.
 Qed.
 
 Lemma step_correct_expr: forall e: Expr, forall x0 y0: Z, forall progs: list Instr, forall st: list Z,
-  (evalInstr ((compile_expr e) ++ progs) st x0 y0) = (evalInstr progs ((evalExpr e x0 y0) :: st) x0 y0).
+  (eval_instr ((compile_expr e) ++ progs) st x0 y0) = (eval_instr progs ((eval_expr e x0 y0) :: st) x0 y0).
 Proof.
   induction e.
   - (*Num*) auto.
@@ -173,19 +173,19 @@ Proof.
   - (*VarY*) auto.
   - (*IteZero*) intros x0 y0 progs st.
     simpl (compile_expr (IteZero e1 e2 e3) ++ progs). repeat rewrite <- app_assoc. rewrite IHe3. rewrite IHe2. rewrite IHe1.
-    simpl (evalInstr ([ICondPick] ++ progs) (evalExpr e1 x0 y0 :: evalExpr e2 x0 y0 :: evalExpr e3 x0 y0 :: st) x0 y0).
-    destruct (evalExpr e1 x0 y0) eqn:condLeft.
-    all: try simpl (evalInstr progs (evalExpr (IteZero e1 e2 e3) x0 y0 :: st) x0 y0).
-    * rewrite -> condLeft. try rewrite Z.mul_0_l. simpl. destruct (evalExpr e2 x0 y0). all:repeat auto.
-    * rewrite -> condLeft. try rewrite Z.mul_0_l. simpl. destruct (evalExpr e3 x0 y0). all:reflexivity.
-    * simpl. destruct (evalExpr e1 x0 y0).
+    simpl (eval_instr ([ICondPick] ++ progs) (eval_expr e1 x0 y0 :: eval_expr e2 x0 y0 :: eval_expr e3 x0 y0 :: st) x0 y0).
+    destruct (eval_expr e1 x0 y0) eqn:condLeft.
+    all: try simpl (eval_instr progs (eval_expr (IteZero e1 e2 e3) x0 y0 :: st) x0 y0).
+    * rewrite -> condLeft. try rewrite Z.mul_0_l. simpl. destruct (eval_expr e2 x0 y0). all:repeat auto.
+    * rewrite -> condLeft. try rewrite Z.mul_0_l. simpl. destruct (eval_expr e3 x0 y0). all:reflexivity.
+    * simpl. destruct (eval_expr e1 x0 y0).
       + discriminate. + reflexivity. + reflexivity.
 Qed.
 
 Lemma step_correct_stmt: forall s: Stmt, forall x0 y0: Z, forall progs: list Instr, forall st: list Z,
-  let e1 := (evalInstr ((compile_stmt s) ++ progs) st x0 y0) in
-  let evt0 := (evalStmt s x0 y0) in
-  let e2 := (evalInstr progs st x0 y0) in
+  let e1 := (eval_instr ((compile_stmt s) ++ progs) st x0 y0) in
+  let evt0 := (eval_stmt s x0 y0) in
+  let e2 := (eval_instr progs st x0 y0) in
   let l := match e1 with
            | None => None
            | Some(_, evt, _) => Some(evt)
@@ -211,36 +211,36 @@ Proof.
     intros x0 y0 progs st.
     assert (((compile_expr e ++ [IWrite; IPop]) ++ progs) = (compile_expr e ++ [IWrite; IPop] ++ progs)) as H.
     + rewrite app_assoc. reflexivity.
-    + rewrite H. rewrite step_correct_expr. simpl. destruct (evalInstr progs st x0 y0) as [p|].
+    + rewrite H. rewrite step_correct_expr. simpl. destruct (eval_instr progs st x0 y0) as [p|].
       * destruct p. destruct p. destruct p0. reflexivity.
       * reflexivity.
   - (*Seq*) simpl in IHs1. simpl in IHs2. intros x0 y0 progs st. simpl.
-    rewrite <- app_assoc. rewrite IHs1. destruct_with_eqn (evalInstr (compile_stmt s2 ++ progs) st x0 y0).
-    destruct_with_eqn (evalInstr progs st x0 y0).
+    rewrite <- app_assoc. rewrite IHs1. destruct_with_eqn (eval_instr (compile_stmt s2 ++ progs) st x0 y0).
+    destruct_with_eqn (eval_instr progs st x0 y0).
     + specialize (IHs2 x0 y0 progs st). rewrite Heqo in IHs2. rewrite Heqo0 in IHs2.
       destruct_with_eqn p. destruct_with_eqn p0. destruct_with_eqn p1. destruct_with_eqn p3. rewrite <- app_assoc. inversion IHs2.
       reflexivity.
     + destruct p. exfalso. specialize (IHs2 x0 y0 progs st). rewrite Heqo in IHs2. rewrite Heqo0 in IHs2. destruct p in IHs2. inversion IHs2.
-    + specialize (IHs2 x0 y0 progs st). rewrite Heqo in IHs2. destruct_with_eqn (evalInstr progs st x0 y0).
+    + specialize (IHs2 x0 y0 progs st). rewrite Heqo in IHs2. destruct_with_eqn (eval_instr progs st x0 y0).
       ++ destruct_with_eqn p. exfalso. destruct p0 in IHs2. inversion IHs2.
       ++ reflexivity.
 Qed.
 
 Theorem compiler_correct: forall s: Stmt, forall x0 y0: Z, forall st: list Z,
   exists st': list Z, exists x0' y0': Z,
-  evalInstr (compile_stmt s) st x0 y0 = Some(st', evalStmt s x0 y0, (x0', y0')).
+  eval_instr (compile_stmt s) st x0 y0 = Some(st', eval_stmt s x0 y0, (x0', y0')).
 Proof.
   assert (forall s: Stmt, forall x0 y0: Z, forall st: list Z,
-      evalInstr (compile_stmt s ++ []) st x0 y0 = evalInstr (compile_stmt s) st x0 y0).
+      eval_instr (compile_stmt s ++ []) st x0 y0 = eval_instr (compile_stmt s) st x0 y0).
   - intros. rewrite app_nil_r. reflexivity.
-  - intros. setoid_rewrite <- H. destruct_with_eqn (evalInstr (compile_stmt s ++ []) st x0 y0).
+  - intros. setoid_rewrite <- H. destruct_with_eqn (eval_instr (compile_stmt s ++ []) st x0 y0).
     + destruct p eqn:Hp.
       pose proof (step_correct_stmt s x0 y0 [] st) as HC. simpl in HC.
       rewrite Heqo in HC. simpl in HC.
       revert HC. destruct p0 eqn:HCp0. intros.
       rewrite app_nil_r in HC.
       inversion HC. rewrite <- H1. exists l. destruct p1. exists z. exists z0. reflexivity.
-    + exfalso. destruct (evalInstr (compile_stmt s ++ []) st x0 y0) eqn:? in Heqo.
+    + exfalso. destruct (eval_instr (compile_stmt s ++ []) st x0 y0) eqn:? in Heqo.
       ++ inversion Heqo.
       ++ pose proof (step_correct_stmt s x0 y0 [] st) as HC. rewrite Heqo0 in HC. simpl in HC. inversion HC.
 Qed.
@@ -266,7 +266,7 @@ Fixpoint link_to_context (s: Stmt) (ctx: StmtContext): Stmt :=
   | CSeqR s' ctx' => Seq s' (link_to_context s ctx')
   end.
 
-Example LE1: (evalInstr (compile_stmt (link_to_context (Write VarX) (CLetX (Num 1) (CSeqR (Write VarX) (CLetX (Num 2) CHole))))) [] 99%Z 99%Z)
+Example LE1: (eval_instr (compile_stmt (link_to_context (Write VarX) (CLetX (Num 1) (CSeqR (Write VarX) (CLetX (Num 2) CHole))))) [] 99%Z 99%Z)
            = Some([], [1%Z; 2%Z], (99%Z, 99%Z)).
 Proof. auto.
 Qed.
@@ -276,18 +276,60 @@ Definition instr_trace_equiv (t1 t2: option (list Z * list Z * (Z * Z))): Prop :
       (t1 = Some(f0, ans, r0)) /\ (t2 = Some(f1, ans, r1)))
     \/ (t1 = None /\ t2 = None).
 
-(* we currently only prepend c1. future work may allow appending c2.*)
+Definition context_equivalence_instr (p1 p2: list Instr): Prop :=
+  forall c1 c2: list Instr, forall st: list Z, forall x y: Z,
+    instr_trace_equiv (eval_instr (c1 ++ p1 ++ c2) st x y) (eval_instr (c1 ++ p2 ++ c2) st x y).
+
 Definition context_equivalence_instr' (p1 p2: list Instr): Prop :=
   forall c1: list Instr, forall st: list Z, forall x y: Z,
-    instr_trace_equiv (evalInstr (c1 ++ p1) st x y) (evalInstr (c1 ++ p2) st x y).
+    instr_trace_equiv (eval_instr (c1 ++ p1) st x y) (eval_instr (c1 ++ p2) st x y).
 
 Definition context_equivalence_stmt (s1 s2: Stmt): Prop :=
   forall ctx: StmtContext, forall x y: Z,
-    (evalStmt (link_to_context s1 ctx) x y) = (evalStmt (link_to_context s2 ctx) x y).
+    (eval_stmt (link_to_context s1 ctx) x y) = (eval_stmt (link_to_context s2 ctx) x y).
 
 
 (* Part 1 of full abstraction *)
 Theorem equivalence_reflection: forall p1 p2: list Instr, forall s1 s2: Stmt,
+  (compile_stmt s1 = p1) /\ (compile_stmt s2 = p2) /\ (context_equivalence_instr p1 p2) -> (context_equivalence_stmt s1 s2).
+Proof.
+  intros. destruct H as [H1]. destruct H as [H2].
+  unfold context_equivalence_instr in H.
+  unfold context_equivalence_stmt. intros.
+  revert y. revert x.
+
+  assert (forall X: Type, forall a b c: list X, a = b -> a ++ c = b ++ c) as app_elim_r.
+  induction c.
+  intros. repeat rewrite app_nil_r. easy.
+  intros. rewrite <- rev_involutive. rewrite distr_rev.
+    rewrite <- (rev_involutive (a ++ a0 :: c)). rewrite distr_rev. rewrite H0. easy.
+
+  assert (forall X: Type, forall a b c: list X, a = b -> c ++ a = c ++ b) as app_elim_l.
+  intros. induction c.
+  easy. repeat rewrite <- app_comm_cons. rewrite IHc. easy.
+
+  induction ctx.
+  + intros. unfold link_to_context.
+    pose proof (compiler_correct s1 x y []) as HC1. destruct HC1 as [st1 [x0 [y0 H0]]].
+    rewrite H1 in H0.
+    pose proof (compiler_correct s2 x y []) as HC2. destruct HC2 as [st2 [x0' [y0' H3]]]. rewrite H2 in H3.
+
+    assert (instr_trace_equiv (eval_instr p1 [] x y) (eval_instr p2 [] x y)).
+    rewrite <- (app_nil_l p1). rewrite <- (app_nil_l p2).
+    rewrite <- (app_nil_r p1). rewrite <- (app_nil_r p2).
+    apply (H [] []). rewrite H0 in H4. rewrite H3 in H4. inversion H4.
+    destruct H5 as [f0 [f1 [ans [r0 [r1 [H5]]]]]]. injection H5. injection H6.
+    intros. rewrite H8. easy. exfalso. destruct H5. easy.
+  + simpl. easy.
+  + simpl. intros. apply (IHctx (eval_expr e x y) y).
+  + simpl. intros. apply (IHctx x (eval_expr e x y)).
+  + simpl. intros. apply app_elim_r. apply IHctx.
+  + simpl. intros. apply app_elim_l. apply IHctx.
+Qed.
+
+
+(* Part 1 of full abstraction *)
+Theorem equivalence_reflection': forall p1 p2: list Instr, forall s1 s2: Stmt,
   (compile_stmt s1 = p1) /\ (compile_stmt s2 = p2) /\ (context_equivalence_instr' p1 p2) -> (context_equivalence_stmt s1 s2).
 Proof.
   intros. destruct H as [H1]. destruct H as [H2].
@@ -311,21 +353,21 @@ Proof.
     rewrite H1 in H0.
     pose proof (compiler_correct s2 x y []) as HC2. destruct HC2 as [st2 [x0' [y0' H3]]]. rewrite H2 in H3.
 
-    assert (instr_trace_equiv (evalInstr p1 [] x y) (evalInstr p2 [] x y)).
+    assert (instr_trace_equiv (eval_instr p1 [] x y) (eval_instr p2 [] x y)).
     rewrite <- (app_nil_l p1). rewrite <- (app_nil_l p2).
     apply (H [] []). rewrite H0 in H4. rewrite H3 in H4. inversion H4.
     destruct H5 as [f0 [f1 [ans [r0 [r1 [H5]]]]]]. injection H5. injection H6.
     intros. rewrite H8. easy. exfalso. destruct H5. easy.
   + simpl. easy.
-  + simpl. intros. apply (IHctx (evalExpr e x y) y).
-  + simpl. intros. apply (IHctx x (evalExpr e x y)).
+  + simpl. intros. apply (IHctx (eval_expr e x y) y).
+  + simpl. intros. apply (IHctx x (eval_expr e x y)).
   + simpl. intros. apply app_elim_r. apply IHctx.
   + simpl. intros. apply app_elim_l. apply IHctx.
 Qed.
 
 Lemma prefix_removal: forall p1 p2 c1: list Instr,
-  (forall st: list Z, forall x y: Z, instr_trace_equiv (evalInstr p1 st x y) (evalInstr p2 st x y)) -> 
-  (forall st': list Z, forall x' y': Z, instr_trace_equiv (evalInstr (c1 ++ p1) st' x' y') (evalInstr (c1 ++ p2) st' x' y')).
+  (forall st: list Z, forall x y: Z, instr_trace_equiv (eval_instr p1 st x y) (eval_instr p2 st x y)) -> 
+  (forall st': list Z, forall x' y': Z, instr_trace_equiv (eval_instr (c1 ++ p1) st' x' y') (eval_instr (c1 ++ p2) st' x' y')).
 Proof.
   intros p1 p2 c1. intros IH0.
   induction c1.
@@ -346,12 +388,12 @@ Proof.
       Transparent instr_trace_equiv. destruct st'.
       unfold instr_trace_equiv. right. easy.
       
-      assert (instr_trace_equiv (evalInstr (c1 ++ p1) (z::st') x' y')
-                                (evalInstr (c1 ++ p2) (z::st') x' y')) as IHc1'.
+      assert (instr_trace_equiv (eval_instr (c1 ++ p1) (z::st') x' y')
+                                (eval_instr (c1 ++ p2) (z::st') x' y')) as IHc1'.
       apply IHc1.
 
-      destruct (evalInstr (c1 ++ p1) (z :: st') x' y') eqn:HL.
-      destruct (evalInstr (c1 ++ p2) (z :: st') x' y') eqn:HR.
+      destruct (eval_instr (c1 ++ p1) (z :: st') x' y') eqn:HL.
+      destruct (eval_instr (c1 ++ p2) (z :: st') x' y') eqn:HR.
       destruct p eqn:?. destruct p0 eqn:?.
       destruct p3 eqn:?. destruct p4 eqn:?. destruct p5 eqn:?. destruct p6 eqn:?.
       unfold instr_trace_equiv in IHc1'.
@@ -376,6 +418,135 @@ Proof.
       destruct st' eqn:?. unfold instr_trace_equiv. right. easy. apply IHc1.
 Qed.
 
+Lemma small_step_instr_none: forall p p': list Instr,
+                        forall x0 y0 x1 y1: Z, forall st0 st1 w1: list Z,
+  ((eval_instr p st0 x0 y0 = Some(st1, w1, (x1, y1))) /\ (eval_instr p' st1 x1 y1 = None))
+    -> (eval_instr (p ++ p') st0 x0 y0 = None).
+Proof.
+  intros p p'. induction p. induction p'.
+  - rewrite app_nil_l. simpl. intros. destruct H. injection H. intros. rewrite H1. rewrite H2. rewrite H4. rewrite H0.
+    easy.
+  - rewrite app_nil_l. intros. destruct H. simpl in H. inversion H. rewrite H0. easy.
+  - intros. destruct H. destruct a.
+    + simpl. destruct st0. exfalso. simpl in H. easy. destruct st0. exfalso. simpl in H. easy.
+             apply (IHp x0 y0 x1 y1 ((z0+z)%Z :: st0) st1 w1). easy.
+    + simpl. destruct st0. exfalso. simpl in H. easy. destruct st0. exfalso. simpl in H. easy.
+             apply (IHp x0 y0 x1 y1 ((z0-z)%Z :: st0) st1 w1). easy.
+    + simpl. destruct st0. exfalso. simpl in H. easy. destruct st0. exfalso. easy. destruct st0. exfalso. easy.
+      destruct z. * apply (IHp x0 y0 x1 y1 (z0 :: st0) st1 w1). easy.
+                  * apply (IHp x0 y0 x1 y1 (z1 :: st0) st1 w1). easy.
+                  * apply (IHp x0 y0 x1 y1 (z1 :: st0) st1 w1). easy.
+    + simpl. destruct st0. exfalso. simpl in H. easy.
+             simpl in H. destruct (eval_instr p (z :: st0) x0 y0) eqn:HP0. destruct p0 eqn:HP1.
+             destruct p1 eqn:HP2. destruct p2 eqn:HP3. inversion H.
+             * destruct (eval_instr (p ++ p') (z :: st0) x0 y0) eqn:HP4.
+               ++ rewrite H2 in HP0. rewrite H4 in HP0. rewrite H5 in HP0. assert (HP0':=conj HP0 H0).
+                  apply (IHp x0 y0 x1 y1 (z::st0) st1 l0) in HP0'. rewrite HP4 in HP0'.
+                  destruct p3 eqn:H6. destruct p4 eqn:H7. destruct p5 eqn:H8. inversion HP0'.
+               ++ easy.
+             * exfalso. easy.
+    + simpl. destruct st0. exfalso. simpl in H. easy. apply (IHp z y0 x1 y1 st0 st1 w1). easy.
+    + simpl. destruct st0. exfalso. simpl in H. easy. apply (IHp x0 z x1 y1 st0 st1 w1). easy.
+    + simpl. destruct st0. exfalso. simpl in H. easy. apply (IHp x0 y0 x1 y1 st0 st1 w1). easy.
+    + simpl. destruct st0. apply (IHp x0 y0 x1 y1 [x0] st1 w1). easy.
+                           apply (IHp x0 y0 x1 y1 (x0::z::st0) st1 w1). easy.
+    + simpl. destruct st0. apply (IHp x0 y0 x1 y1 [y0] st1 w1). easy.
+                           apply (IHp x0 y0 x1 y1 (y0::z::st0) st1 w1). easy.
+    + simpl. destruct st0. apply (IHp x0 y0 x1 y1 [z] st1 w1). easy.
+                           apply (IHp x0 y0 x1 y1 (z::z0::st0) st1 w1). easy.
+    + simpl. destruct st0. exfalso. simpl in H. easy. apply (IHp x0 y0 x1 y1 (z::z::st0) st1 w1). easy.
+    + simpl. destruct st0. exfalso. simpl in H. easy. destruct st0. exfalso. simpl in H. easy.
+             apply (IHp x0 y0 x1 y1 (z0::z::st0) st1 w1). easy.
+Qed.
+
+Lemma small_step_instr_some: forall p p': list Instr,
+                        forall x0 y0 x1 y1 x2 y2: Z, forall st0 st1 st2 w1 w2: list Z,
+  ((eval_instr p st0 x0 y0 = Some(st1, w1, (x1, y1))) /\ (eval_instr p' st1 x1 y1 = Some(st2, w2, (x2, y2))))
+    -> (eval_instr (p ++ p') st0 x0 y0 = Some(st2, w1 ++ w2, (x2, y2))).
+Proof.
+  intros p p'. induction p. induction p'.
+  - rewrite app_nil_l. simpl. intros. destruct H. injection H. intros. rewrite H1. rewrite H2. rewrite H4. rewrite H0.
+    rewrite <- H3. rewrite app_nil_l. easy.
+  - rewrite app_nil_l. intros. destruct H. simpl in H. inversion H. rewrite H0.
+    rewrite app_nil_l. easy.
+  - intros. destruct H. destruct a.
+    + simpl. destruct st0. exfalso. simpl in H. easy. destruct st0. exfalso. simpl in H. easy.
+             apply (IHp x0 y0 x1 y1 x2 y2 ((z0+z)%Z :: st0) st1 st2).
+             * easy.
+    + simpl. destruct st0. exfalso. simpl in H. easy. destruct st0. exfalso. simpl in H. easy.
+             apply (IHp x0 y0 x1 y1 x2 y2 ((z0-z)%Z :: st0) st1 st2).
+             * easy.
+    + simpl. destruct st0. exfalso. simpl in H. easy. destruct st0. exfalso. easy. destruct st0. exfalso. easy.
+      destruct z. * apply (IHp x0 y0 x1 y1 x2 y2 (z0 :: st0) st1 st2). easy.
+                  * apply (IHp x0 y0 x1 y1 x2 y2 (z1 :: st0) st1 st2). easy.
+                  * apply (IHp x0 y0 x1 y1 x2 y2 (z1 :: st0) st1 st2). easy.
+    + simpl. destruct st0. exfalso. simpl in H. easy.
+             simpl in H. destruct (eval_instr p (z :: st0) x0 y0) eqn:HP0. destruct p0 eqn:HP1.
+             destruct p1 eqn:HP2. destruct p2 eqn:HP3. inversion H.
+             * destruct (eval_instr (p ++ p') (z :: st0) x0 y0) eqn:HP4.
+               ++ rewrite H2 in HP0. rewrite H4 in HP0. rewrite H5 in HP0. assert (HP0':=conj HP0 H0).
+                  apply (IHp x0 y0 x1 y1 x2 y2 (z::st0) st1 st2 l0 w2) in HP0'. rewrite HP4 in HP0'.
+                  destruct p3 eqn:H6. destruct p4 eqn:H7. destruct p5 eqn:H8. inversion HP0'.
+                  rewrite app_comm_cons. easy.
+               ++ exfalso. rewrite H2 in HP0. rewrite H4 in HP0. rewrite H5 in HP0. assert (HP0':=conj HP0 H0).
+                  apply (IHp x0 y0 x1 y1 x2 y2 (z::st0) st1 st2 l0 w2) in HP0'. rewrite HP4 in HP0'. easy.
+             * exfalso. easy.
+    + simpl. destruct st0. exfalso. simpl in H. easy. apply (IHp z y0 x1 y1 x2 y2 st0 st1 st2). easy.
+    + simpl. destruct st0. exfalso. simpl in H. easy. apply (IHp x0 z x1 y1 x2 y2 st0 st1 st2). easy.
+    + simpl. destruct st0. exfalso. simpl in H. easy. apply (IHp x0 y0 x1 y1 x2 y2 st0 st1 st2). easy.
+    + simpl. destruct st0. apply (IHp x0 y0 x1 y1 x2 y2 [x0] st1 st2). easy.
+                           apply (IHp x0 y0 x1 y1 x2 y2 (x0::z::st0) st1 st2). easy.
+    + simpl. destruct st0. apply (IHp x0 y0 x1 y1 x2 y2 [y0] st1 st2). easy.
+                           apply (IHp x0 y0 x1 y1 x2 y2 (y0::z::st0) st1 st2). easy.
+    + simpl. destruct st0. apply (IHp x0 y0 x1 y1 x2 y2 [z] st1 st2). easy.
+                           apply (IHp x0 y0 x1 y1 x2 y2 (z::z0::st0) st1 st2). easy.
+    + simpl. destruct st0. exfalso. simpl in H. easy. apply (IHp x0 y0 x1 y1 x2 y2 (z::z::st0) st1 st2). easy.
+    + simpl. destruct st0. exfalso. simpl in H. easy. destruct st0. exfalso. simpl in H. easy.
+             apply (IHp x0 y0 x1 y1 x2 y2 (z0::z::st0) st1 st2). easy.
+Qed.
+
+Axiom step_stuck_safety: forall p p': list Instr, forall x0 y0: Z, forall st0: list Z,
+  (eval_instr p st0 x0 y0 = None) -> (eval_instr (p ++ p') st0 x0 y0 = None).
+
+Lemma suffix_removal: forall p1 p2 c2: list Instr,
+  (forall st: list Z, forall x y: Z, (eval_instr p1 st x y) = (eval_instr p2 st x y)) -> 
+  (forall st': list Z, forall x' y': Z, instr_trace_equiv (eval_instr (p1 ++ c2) st' x' y') (eval_instr (p2 ++ c2) st' x' y')).
+Proof.
+  intros.
+  destruct (eval_instr p1 st' x' y') eqn:HP1. destruct p as [[st_p1_end w_p1_end] [x_p1_end y_p1_end]] eqn:?.
+  destruct (eval_instr c2 st_p1_end x_p1_end y_p1_end) eqn:Hc.
+  destruct p0 as [[st_c_end1 w_c_end1] [x_c_end1 y_c_end1]] eqn:?.
+  pose proof (small_step_instr_some p1 c2 x' y' x_p1_end y_p1_end x_c_end1 y_c_end1 st' st_p1_end st_c_end1 w_p1_end w_c_end1).
+  assert (HPc1 := conj HP1 Hc). apply H0 in HPc1. clear H0.
+  rewrite HPc1. destruct (eval_instr p2 st' x' y') eqn:HP2. destruct p3 as [[st_p2_end w_p2_end] [x_p2_end y_p2_end]] eqn:?.
+  destruct (eval_instr c2 st_p2_end x_p2_end y_p2_end) eqn:Hc'.
+  { destruct p4 as [[st_c_end2 w_c_end2] [x_c_end2 y_c_end2]] eqn:?.
+    assert (HPc2 := conj HP2 Hc').
+    pose proof (small_step_instr_some p2 c2 x' y' x_p2_end y_p2_end x_c_end2 y_c_end2 st' st_p2_end st_c_end2 w_p2_end w_c_end2) as H0'.
+    apply H0' in HPc2. clear H0'. rewrite HPc2. 
+    specialize (H st' x' y').
+    rewrite HP1 in H. rewrite HP2 in H. inversion H.
+    unfold instr_trace_equiv. left. exists st_c_end1. exists st_c_end2. exists (w_p2_end ++ w_c_end1).
+    exists (x_c_end1, y_c_end1). exists (x_c_end2, y_c_end2). split. easy. rewrite H1 in Hc. rewrite H3 in Hc. rewrite H4 in Hc.
+    rewrite Hc' in Hc. inversion Hc. easy.
+  }
+  - exfalso. specialize (H st' x' y'). rewrite <- H in HP2. rewrite HP1 in HP2. inversion HP2.
+    rewrite <- H1 in Hc'. rewrite <- H3 in Hc'. rewrite <- H4 in Hc'. rewrite Hc in Hc'. easy.
+  - exfalso. specialize (H st' x' y'). rewrite <- H in HP2. rewrite HP1 in HP2. inversion HP2.
+  - specialize (H st' x' y'). destruct (eval_instr p2 st' x' y') eqn:HP2. destruct p0 as [[st_p2_end w_p2_end] [x_p2_end y_p2_end]] eqn:?.
+     * rewrite HP1 in H. inversion H.
+       pose proof (small_step_instr_none p1 c2 x' y' x_p1_end y_p1_end st' st_p1_end w_p1_end).
+       assert (HPc1 := conj HP1 Hc). apply H0 in HPc1. rewrite HPc1.
+       pose proof (small_step_instr_none p2 c2 x' y' x_p2_end y_p2_end st' st_p2_end w_p2_end) as H0'.
+       rewrite H1 in Hc. rewrite H3 in Hc. rewrite H4 in Hc. assert (HPc2 := conj HP2 Hc). 
+       apply H0' in HPc2. rewrite HPc2. unfold instr_trace_equiv. right. easy.
+     * rewrite HP1 in H. inversion H.
+  - specialize (H st' x' y'). destruct (eval_instr p2 st' x' y') eqn:HP2. destruct p as [[st_p2_end w_p2_end] [x_p2_end y_p2_end]] eqn:?.
+     * rewrite HP1 in H. inversion H.
+     * pose proof (step_stuck_safety p1 c2 x' y' st'). apply H0 in H. rewrite H.
+       pose proof (step_stuck_safety p2 c2 x' y' st'). apply H1 in HP2. rewrite HP2. unfold instr_trace_equiv. right. easy.
+Qed.
+
 (* Part 2 of full abstraction *)
 Theorem equivalence_preservation': forall p1 p2: list Instr, forall s1 s2: Stmt,
   (compile_stmt s1 = p1) /\ (compile_stmt s2 = p2) /\ (context_equivalence_stmt s1 s2) -> (context_equivalence_instr' p1 p2).
@@ -389,10 +560,22 @@ Proof.
   rewrite H1 in Hs1. rewrite H in Hs2. rewrite H3 in Hs1.
   destruct Hs1 as [st' [x0' [y0' Hs1]]].
   destruct Hs2 as [st'' [x0'' [y0'' Hs2]]].
-  rewrite Hs1. rewrite Hs2. unfold instr_trace_equiv. left.
-  exists st'. exists st''. exists (evalStmt s2 x y). exists (x0', y0'). exists (x0'', y0'').
-  easy. 
+  (*apply suffix_removal. intros.
+  pose proof (H2 CHole x0 y0) as H3'. unfold link_to_context in H3'.
+  pose proof (compiler_correct s1 x0 y0 st1) as Hs1'. pose proof (compiler_correct s2 x0 y0 st1) as Hs2'.
+  rewrite H1 in Hs1'. rewrite H in Hs2'. rewrite H3' in Hs1'.
+  destruct Hs1' as [st_' [x0_' [y0_' Hs1']]].
+  destruct Hs2' as [st_'' [x0_'' [y0_'' Hs2']]].*)
+  unfold instr_trace_equiv. left. exists st'. exists st''. exists (eval_stmt s2 x y). exists (x0', y0'). exists (x0'', y0'').
+  split. easy. easy.
 Qed.
 
+Theorem full_abstraction': forall p1 p2: list Instr, forall s1 s2: Stmt,
+  ((compile_stmt s1 = p1) /\ (compile_stmt s2 = p2)) -> ((context_equivalence_stmt s1 s2) <-> (context_equivalence_instr' p1 p2)).
+Proof.
+  intros. split. 
+  - intros. apply (equivalence_preservation' p1 p2 s1 s2). split. easy. easy.
+  - intros. apply (equivalence_reflection' p1 p2 s1 s2). split. easy. easy.
+Qed.
 
 
